feat(Vstd): refactor continuing for Set

VerusLean/Vstd/Set/Defs.lean
@@ -6,19 +6,35 @@ namespace Vstd
 /--
   Verus finite Sets.
 
-  This is a true shim layer: replace the underlying definitions,
-  and prove that they obey the minimal set of theorems at the end of the file.
-  Then all theorems in `Set.Basic.lean` should be proven.
+  The definitions and theorems in this file are intended to be a shim layer:
+  replace the definitions and theorems marked as SHIM, and the remaining
+  theorems in this file and in `Basic.lean` should prove automatically.
 
-  These `Set`s need to be `inductive`, or else other inductive types
-  struggle to prove termination, e.g., with
-
+  Note: whatever definition you use for `Set` needs to be `inductive`,
+  or else other inductive types will struggle to prove termination.
+  For example,
   ```
   inductive MyType where
   | mk : (s : Set MyType) → MyType
   ```
+
+  List of SHIM functions:
+    - `empty`
+    - `singleton`
+    - `card`
+    - `ofList`
+    - `toList`
+    - `bmem`    (if you prefer a `Bool`-based view of Sets)
+    - `bsubset` (if you prefer a `Bool`-based view of Sets)
+    - `beq`     (if you prefer a `Bool`-based view of Sets)
+    - `mem`     (pure membership, not `bmem`)
+    - `choose`
+    - `insert`, `remove`
+    - `union`, `inter`, `sdiff`  (Set algebra)
+    - `map`, `filter`, `fold`    (Higher-order functions)
 -/
 
+-- SHIM
 inductive Set (α : Type u) : Type u
   -- If swapping out implementations, refer to something else here
   | mk (s : List α) : Set α
@@ -27,6 +43,7 @@ namespace Set
 
 variable {α : Type u} {β : Type v} {γ : Type w}
 
+-- SHIM
 def empty : Set α :=
   mk []
 
@@ -36,25 +53,38 @@ instance instInhabited : Inhabited (Set α) where
 instance instEmptyCollection : EmptyCollection (Set α) where
   emptyCollection := Set.empty
 
+-- SHIM
 def singleton (a : α) : Set α :=
   mk [a]
 
 instance instSingleton : Singleton α (Set α) where
   singleton := Set.singleton
 
-def card (s : Set α) : Nat :=
+-- SHIM
+-- This non-trivial implementation is due to the list maybe having duplicates
+-- One way to make this simpler is to make the other definitions more complicated.
+-- For example, instead of `union` being `List.append` under the hood,
+-- do a `fold` across `insert`, which checks for duplicates
+def card [DecidableEq α] (s : Set α) : Nat :=
   match s with
-  | mk l => l.length
+  | mk l =>
+    match l with
+    | [] => 0
+    | (x :: xs) =>
+      if x ∈ xs then card (mk xs)
+      else card (mk xs) + 1
 
 /-
   CC: In some sense, including these two functions are sufficient to define
       all other functions. Just convert the set into a List, and then
       use a List function. Maybe this is the right approach...
 -/
+-- SHIM
 def ofList (l : List α) : Set α :=
   mk l
 
 -- CC: No guarantees on ordering, or the inclusion of duplicates.
+-- SHIM
 def toList (s : Set α) : List α :=
   match s with
   | mk l => l
@@ -77,10 +107,12 @@ section BoolOps
 variable [BEq α]
 
 -- The order of the arguments is reversed from the `Membership` class
+-- SHIM
 def bmem (s : Set α) (a : α) : Bool :=
   match s with
   | mk l => l.contains a
 
+-- SHIM
 def bsubset (s₁ s₂ : Set α) : Bool :=
   match s₁, s₂ with
   | mk l₁, mk l₂ => l₁.all (l₂.contains ·)
@@ -95,8 +127,18 @@ def bsubset (s₁ s₂ : Set α) : Bool :=
 def beq (s₁ s₂ : Set α) : Bool :=
   s₁.bsubset s₂ && s₂.bsubset s₁
 
+/-
+
+Uncomment this if `bmem` is the preferred definition.
+
+def mem (s : Set α) (a : α) : Prop :=
+  s.bmem a
+-/
+
 end BoolOps /- section -/
 
+-- This is the non-`bmem`-based definition
+-- SHIM
 def mem (s : Set α) (a : α) : Prop :=
   match s with
   | mk l => a ∈ l
@@ -112,8 +154,7 @@ instance instDecidableMembership [DecidableEq α] (a : α) (s : Set α) : Decida
     · apply isFalse h
 
 def subset (s₁ s₂ : Set α) : Prop :=
-  match s₁, s₂ with
-  | mk l₁, mk l₂ => ∀ x ∈ l₁, x ∈ l₂
+  ∀ x ∈ s₁, x ∈ s₂
 
 instance instHasSubset : HasSubset (Set α) where
   Subset := subset
@@ -122,8 +163,7 @@ instance instLE : LE (Set α) where
   le := subset
 
 def disjoint (s₁ s₂ : Set α) : Prop :=
-  match s₁, s₂ with
-  | mk l₁, mk l₂ => ∀ x ∈ l₁, x ∉ l₂
+  ∀ x ∈ s₁, x ∉ s₂
 
 -- CC: Because we don't have a canonical sorting function,
 --     we can't define equality with "strict equality".
@@ -132,6 +172,7 @@ def disjoint (s₁ s₂ : Set α) : Prop :=
 def ext_eq (s₁ s₂ : Set α) : Prop :=
   s₁ ⊆ s₂ ∧ s₂ ⊆ s₁
 
+-- SHIM (because the way we choose an element is dependent on the underlying data structure)
 def choose (s : Set α) [Inhabited α] : α :=
   match s with
   | mk [] => default
@@ -139,13 +180,19 @@ def choose (s : Set α) [Inhabited α] : α :=
 
 /- # functions that modify the sets -/
 
--- Blindly insert the element. Who cares about duplicates!
+/-
+  (Almost) all of these functions are marked as "SHIM"
+  because their implementations depend on the underlying data structure.
+-/
+
+-- SHIM
+-- Insert the element, only if it isn't a duplicate
 -- CC: Alternatively, implement a `binsert` that depends on `BEq α`.
 --     The problem with this is that this requires you to implement `bunion`, `binter`, etc.
 --     Essentially, the whole set of boolean-based operations, which may not be desirable.
-def insert (s : Set α) (a : α) : Set α :=
+def insert [DecidableEq α] (s : Set α) (a : α) : Set α :=
   match s with
-  | mk l => mk <| a :: l
+  | mk l => if a ∈ l then s else mk <| a :: l
 
 /-
 CC: Alternate implementation
@@ -154,13 +201,16 @@ def insert' [DecidableEq α] (s : Set α) (a : α) : Set α :=
   | mk l => mk <| if a ∈ l then l else a :: l
 -/
 
-instance instInsert : Insert α (Set α) where
+instance instInsert [DecidableEq α] : Insert α (Set α) where
   insert := (fun a s => insert s a)
 
+-- SHIM
 def remove [DecidableEq α] (s : Set α) (a : α) : Set α :=
   match s with
   | mk l => mk <| l.filter (fun x => x ≠ a)
 
+-- SHIM
+-- This keeps around duplicates, but is pretty efficient otherwise
 def union (s₁ s₂ : Set α) : Set α :=
   match s₁, s₂ with
   | mk l₁, mk l₂ => mk <| l₁ ++ l₂
@@ -168,6 +218,7 @@ def union (s₁ s₂ : Set α) : Set α :=
 instance instUnion : Union (Set α) where
   union := union
 
+-- SHIM
 def inter [DecidableEq α] (s₁ s₂ : Set α) : Set α :=
   match s₁, s₂ with
   | mk l₁, mk l₂ => mk <| l₁.filter (fun x => x ∈ l₂)
@@ -175,6 +226,7 @@ def inter [DecidableEq α] (s₁ s₂ : Set α) : Set α :=
 instance instInter [DecidableEq α] : Inter (Set α) where
   inter := inter
 
+-- SHIM
 def sdiff [DecidableEq α] (s₁ s₂ : Set α) : Set α :=
   match s₁, s₂ with
   | mk l₁, mk l₂ => mk <| l₁.filter (fun x => x ∉ l₂)
@@ -185,41 +237,85 @@ instance instSDiff [DecidableEq α] : SDiff (Set α) where
 def symmDiff [DecidableEq α] (s₁ s₂ : Set α) : Set α :=
   (s₁ \ s₂) ∪ (s₂ \ s₁)
 
-/-! # higher order functions -/
+/-! # higher-order functions -/
 
+-- SHIM
 def map (f : α → β) : Set α → Set β :=
   fun | mk l => mk <| l.map f
 
-def mapConst (b : β) : Set α → Set β :=
-  fun | mk l => mk <| l.map (fun _ => b)
+-- Not SHIM, but can be replaced with a more efficient implementation
+def mapConst (b : β) (s : Set α) : Set β :=
+  s.map (fun _ => b)
 
 instance instFunctor : Functor Set where
   map := map
   mapConst := mapConst
 
+-- SHIM
 def filter (s : Set α) (pred : α → Bool) : Set α :=
   match s with
   | mk l => mk <| l.filter pred
 
+-- SHIM
+-- Order and multiplicity of the elements to `f` are not guaranteed,
+-- which means that for correctness, `f` needs to be commutative and idempotent-like.
+def fold (s : Set α) (init : β) (f : β → α → β) : β :=
+  match s with
+  | mk l => l.foldl f init
+
 /-! # correctness theorems -/
 
 /-
-  In this section, keep the theorem names, attributes,
-  and statements, but change the proofs to fit the above definitions.
+  In this section, do not edit the theorem names, attributes, and statements,
+  but do change the proofs to fit the above definitions.
+
+  Core lemmas that will be affected by a change in the underlying data structure
+  are marked SHIM, but depending on what lemmas are imported, some theorems
+  might get proven automatically anyways.
+
+  In this section, we prefer `simp` over `simp only` in SHIM lemmas
+  to increase the odds that switching out the underlying data structure
+  will lead to fewer broken proofs, in case other lemmas on the new
+  underlying data structure are in scope.
 -/
 
+-- SHIM
 @[simp]
 theorem not_mem_empty : ∀ (a : α), a ∉ (∅ : Set α) := by
   intro a h_contra; cases h_contra
 
--- Something is an element of the set if it is a member of the underlying data structure.
--- CC: A bit interface breaking...
+/--
+  Something is an element of the set if it is a member of the underlying data structure.
+
+  SHIM
+
+  Explicitly breaks the API/interface to access the underlying data structure.
+
+  This theorem requires the underlying data structure to support `Membership`,
+  but this isn't too much of an ask. (Anything `List`-based will.)
+
+  We use this lemma to derive other lemmas on membership in this file.
+-/
 theorem mem_iff {a : α} {s : Set α} : a ∈ s ↔ a ∈ (match s with | mk l => l) := by
   rfl
+
+/-
+  CC: If using a `bmem`-based definition, a similar set of starting lemmas are needed
+      to convert to the `Prop`-based functions. But we should prefer the Prop-based
+      functions, to be consistent.
+
+      In fact, we probably will need a `bX_iff_X` for each kind of boolean function.
+
+  SHIM
+-/
+theorem bmem_iff_mem [BEq α] [LawfulBEq α] {a : α} {s : Set α} : s.bmem a ↔ a ∈ s := by
+  match s with
+  | mk l => simp [bmem, mem_iff]
 
 theorem subset_iff {s₁ s₂ : Set α} : s₁ ⊆ s₂ ↔ ∀ a, a ∈ s₁ → a ∈ s₂ := by
   rfl
 
+-- SHIM
 theorem ext_eq_iff {s₁ s₂ : Set α} : ext_eq s₁ s₂ ↔ ∀ a, a ∈ s₁ ↔ a ∈ s₂ := by
   match s₁, s₂ with
   | mk l₁, mk l₂ =>
@@ -230,94 +326,118 @@ theorem ext_eq_iff {s₁ s₂ : Set α} : ext_eq s₁ s₂ ↔ ∀ a, a ∈ s₁
     · intro h
       exact ⟨fun _ ha => (h _).mp ha, fun _ ha => (h _).mpr ha⟩
 
+-- SHIM
 @[simp]
-theorem toList_ofList (l : List α) : toList (ofList l) = l :=
-  rfl
+theorem mem_ofList_iff {a : α} {l : List α} : a ∈ (ofList l : Set α) ↔ a ∈ l := by
+  simp [ofList, mem_iff]
 
+-- SHIM
 @[simp]
-theorem ofList_toList (s : Set α) : ofList (toList s) = s :=
-  rfl
+theorem mem_toList_iff {a : α} {s : Set α} : a ∈ toList s ↔ a ∈ s := by
+  match s with
+  | mk l => simp [toList, mem_iff]
 
 theorem eq_empty_iff {s : Set α} : ext_eq s ∅ ↔ ∀ a, a ∉ s := by
-  match s with
-  | mk l => simp only [ext_eq, subset_iff, not_mem_empty, imp_false,
-                        false_implies, implies_true, and_true]
+  simp only [ext_eq_iff, not_mem_empty, iff_false]
 
+-- SHIM
 @[simp]
 theorem mem_singleton_iff {a b : α} : b ∈ ({a} : Set α) ↔ b = a := by
   simp [Singleton.singleton, singleton, mem_iff]
 
-theorem mem_insert_iff {a b : α} {s : Set α} : b ∈ (s.insert a) ↔ b = a ∨ b ∈ s := by
+-- SHIM
+theorem mem_insert_iff [DecidableEq α] {a b : α} {s : Set α} : b ∈ (s.insert a) ↔ b = a ∨ b ∈ s := by
   match s with
-  | mk l => simp only [insert, mem_iff, List.mem_cons]
+  | mk l =>
+    simp [insert, mem_iff]
+    by_cases h : a ∈ l
+    · simp [h]; rintro rfl; exact h
+    · simp [h]
 
+-- SHIM
 theorem mem_remove_iff [DecidableEq α] {a b : α} {s : Set α}
     : b ∈ (s.remove a) ↔ b ≠ a ∧ b ∈ s := by
   match s with
-  | mk l =>
-    simp only [remove, ne_eq, decide_not, mem_iff, List.mem_filter,
-      Bool.not_eq_eq_eq_not, Bool.not_true, decide_eq_false_iff_not]
-    exact And.comm
+  | mk l => simp [remove, mem_iff]; exact And.comm
 
+-- SHIM
+@[simp]
+theorem card_empty [DecidableEq α] : card (∅ : Set α) = 0 := by
+  simp [card, EmptyCollection.emptyCollection, empty]
+
+-- SHIM
+theorem card_insert [DecidableEq α] (a : α) (s : Set α) :
+    card (s.insert a) = if a ∈ s then card s else card s + 1 := by
+  match s with
+  | mk l =>
+    simp only [insert, mem_iff]
+    by_cases h : a ∈ l
+    · simp [h]
+    · simp [h, card]
+
+-- TODO: Can probably prove all other card_X theorems, but we might need more here
+
+-- SHIM
 theorem choose_mem [Inhabited α] {s : Set α} : (∃ x, x ∈ s) → s.choose ∈ s := by
   intro h
   match s with
-  | mk [] => simp only [mem_iff, List.not_mem_nil, exists_const] at h
-  | mk (a :: _) => simp only [choose, mem_iff, List.mem_cons, true_or]
+  | mk [] => simp [mem_iff, exists_const] at h
+  | mk (a :: _) => simp [choose, mem_iff]
 
+-- SHIM
 theorem mem_union_iff {a : α} {s₁ s₂ : Set α}
     : a ∈ (s₁ ∪ s₂) ↔ a ∈ s₁ ∨ a ∈ s₂ := by
   match s₁, s₂ with
-  | mk l₁, mk l₂ => simp only [union, mem_iff, List.mem_append]
+  | mk l₁, mk l₂ => simp [union, mem_iff]
 
+-- SHIM
 theorem mem_inter_iff [DecidableEq α] {a : α} {s₁ s₂ : Set α}
     : a ∈ (s₁ ∩ s₂) ↔ a ∈ s₁ ∧ a ∈ s₂ := by
   match s₁, s₂ with
-  | mk l₁, mk l₂ => simp only [mem_iff, inter, List.mem_filter, decide_eq_true_eq]
+  | mk l₁, mk l₂ => simp [mem_iff, inter]
 
+-- SHIM
 theorem mem_sdiff_iff [DecidableEq α] {a : α} {s₁ s₂ : Set α}
     : a ∈ (s₁ \ s₂) ↔ a ∈ s₁ ∧ a ∉ s₂ := by
   match s₁, s₂ with
-  | mk l₁, mk l₂ =>
-    simp only [mem_iff, sdiff, decide_not, List.mem_filter,
-      Bool.not_eq_eq_eq_not, Bool.not_true, decide_eq_false_iff_not]
+  | mk l₁, mk l₂ => simp [mem_iff, sdiff]
 
 theorem mem_symmDiff_iff [DecidableEq α] {a : α} {s₁ s₂ : Set α}
     : a ∈ symmDiff s₁ s₂ ↔ (a ∈ s₁ \ s₂ ∨ a ∈ s₂ \ s₁) := by
   simp only [symmDiff, mem_union_iff]
 
 theorem disjoint_iff [DecidableEq α] {s₁ s₂ : Set α} : disjoint s₁ s₂ ↔ ext_eq (s₁ ∩ s₂) ∅ := by
-  match s₁, s₂ with
-  | mk l₁, mk l₂ =>
-    -- CC: Doesn't get to a stable simp normal form here, need to split to two lines
-    simp only [disjoint, eq_empty_iff, mem_inter_iff, not_and]
-    simp only [mem_iff]
+  simp only [disjoint, eq_empty_iff, mem_inter_iff, not_and]
 
 theorem disjoint_iff_not_mem_inter [DecidableEq α] {s₁ s₂ : Set α}
     : disjoint s₁ s₂ ↔ ∀ a, a ∉ (s₁ ∩ s₂) := by
   rw [disjoint_iff, eq_empty_iff]
 
+-- SHIM
 theorem mem_filter_iff {p : α → Bool} {s : Set α} {a : α}
     : a ∈ filter s p ↔ a ∈ s ∧ p a := by
   match s with
-  | mk l => simp only [filter, mem_iff, List.mem_filter]
+  | mk l => simp [filter, mem_iff]
 
+-- SHIM
 theorem mem_map_iff {α β : Type u} {f : α → β} {s : Set α} {b : β}
     : b ∈ f <$> s ↔ ∃ a, a ∈ s ∧ f a = b := by
   match s with
-  | mk l => simp only [map, mem_iff, List.mem_map, exists_prop]
+  | mk l => simp [map, mem_iff]
 
+-- SHIM?
 theorem map_const {α β : Type u}
     : (Functor.mapConst : β → Set α → Set β) = Functor.map ∘ Function.const α := by
   ext b s
-  match s with
-  | mk l => rfl
+  rfl
 
+-- SHIM
 @[simp]
 theorem id_map {α : Type u} (s : Set α) : id <$> s = s := by
   match s with
-  | mk l => simp only [Functor.map, map, List.map_id_fun, id_eq]
+  | mk l => simp [Functor.map, map, id_eq]
 
+-- SHIM
 @[simp]
 theorem comp_map {α β γ : Type u} (g : α → β) (h : β → γ) (s : Set α) :
     (h ∘ g) <$> s = h <$> g <$> s := by
@@ -329,13 +449,63 @@ instance instLawfulFunctor : LawfulFunctor Set where
   id_map := id_map
   comp_map := comp_map
 
+/-! # fold -/
+
+-- SHIM
+@[simp]
+theorem fold_empty (f : β → α → β) (init : β) :
+    fold (∅ : Set α) init f = init := by
+  simp [fold, empty]
+
+/-
+  For correctness, we require that `f` is commutative and idempotent-like.
+-/
+
+class SetFold (f : β → α → β) where
+  comm : ∀ (a₁ a₂ : α) (b : β), f (f b a₁) a₂ = f (f b a₂) a₁
+  idempotent : ∀ (a : α) (b : β), f (f b a) a = f b a
+
+/-
+  CC: TODO. There's a whole bunch of lemmas you could write here.
+      This is an exercise to CZ! Perhaps see what Verus does?
+
+      I'll suggest a few lemmas, but this might not be the best course of action.
+
+      Before you start proving things, convince yourself for why `SetFold`
+      is a necessary well-behavedness assumption to have around.
+      (Perhaps compare and contrast to `FoldCommutative` in `Seq.Defs.lean`)
+-/
+
+-- SHIM
+@[simp]
+theorem fold_insert [DecidableEq α] (s : Set α) (a : α) (f : β → α → β) [SetFold f] (init : β)
+    : fold (insert s a) init f = f (fold s init f) a := by
+  match s with
+  | mk l =>
+    simp [insert, fold]
+    induction l generalizing init with
+    | nil => simp [insert, fold]
+    | cons x xs ih =>
+      stop
+      by_cases h_ax : a = x
+      · subst h_ax
+        simp [SetFold.comm a _, ih (f init a)]
+        done
+
+theorem fold_eq_of_ext_eq {s₁ s₂ : Set α} (f : β → α → β) [SetFold f] (init : β)
+    : ext_eq s₁ s₂ → fold s₁ init f = fold s₂ init f := by
+  sorry
+
 /-! # derived operations and lemmas -/
 
 -- CC: The correctness of the above should imply the correctness of these?
 
-def filterMap {α β : Type u} (f : α → Option β) (s : Set α) : Set β :=
+-- SHIM?
+def filterMap (f : α → Option β) (s : Set α) : Set β :=
   match s with
   | mk l => mk <| l.filterMap f
+
+-- TODO: Define `bany` and `ball`?
 
 def any {α : Type u} (s : Set α) (p : α → Bool) : Prop :=
   ∃ a, a ∈ s ∧ p a
@@ -343,112 +513,32 @@ def any {α : Type u} (s : Set α) (p : α → Bool) : Prop :=
 def all {α : Type u} (s : Set α) (p : α → Bool) : Prop :=
   ∀ a, a ∈ s → p a
 
-#exit
-
-  protected ext (s₁ s₂ : S α) : (∀ (x : α), x ∈ s₁ ↔ x ∈ s₂) → s₁ = s₂
-  disjoint_iff {s₁ s₂ : S α} : disjoint s₁ s₂ ↔ ∀ a, a ∉ s₁ ∩ s₂
-  mem_ofList_iff {a : α} {l : List α} : a ∈ (ofList l : S α) ↔ a ∈ l
-  mem_map_iff {f : α → β} {s : S α} {b : β}
-    : b ∈ f <$> s ↔ ∃ a, a ∈ s ∧ f a = b
-  mem_filterMap_iff {α β : Type u} {f : α → Option β} {s : S α} {b : β}
-    : b ∈ filterMap f s ↔ ∃ a, a ∈ s ∧ f a = some b
-
+-- SHIM
+theorem mem_filterMap_iff {f : α → Option β} {s : Set α} {b : β}
+    : b ∈ filterMap f s ↔ ∃ a, a ∈ s ∧ f a = some b := by
+  match s with
+  | mk l => simp [filterMap, mem_iff]
 
 end Set /- namespace -/
 
+end Vstd
+
 #exit
 
+-- TODO: I've kept anything below this #exit that hasn't been implemented completely above
 
-/--
-  Verus `Vstd` sets.
--/
--- TODO: consider the following approach to make it
--- so in the testfile, either a generic `S` or a specific `Set` can be used?
--- instead of {S: } [], write [S: ]
--- class VSetLikeF
 
 class VSetLikeF (S : Type u → Type v) -- Type u → Type u
   extends
     Functor S
   where
-  map' : {α β : Type u} → (s : S α) → (f : α → β) → S β := fun s f => Functor.map f s
-  mem : {α : Type u} → S α → α → Prop
-  -- mem : {α : Type u} → S α → α → Bool -- if [DecidableEq α] here then Shim.lean can be Cedar's defn, but then not sure how to satisfy `instance instMembership`
-  empty : {α : Type u} → S α -- why is the empty set an infinite set in Verus?
-  insert : {α : Type u} → S α → α → S α
-  remove : {α : Type u} → α → S α → S α
-  singleton : {α : Type u} → α → S α :=
-    fun a => insert empty a
-  -- To get around `noncomputable instance` for `Shim.lean`, we enforce that `α` be inhabited.
-  -- choose {α : Type u} [Inhabited α] : (s : S α) → (h : ∃ x, mem s x) → α
-  /- CZ: How about that we don't require (h : ∃ x, mem s x), and just say we
-     don't care what ∅.choose returns, as long as α is inhabited it's fine -/
-  choose {α : Type u} [Inhabited α] : S α → α
-  subset : {α : Type u} → S α → S α → Prop := -- Cedar's defn is Bool instead of Prop, same below
-    fun s₁ s₂ => ∀ a, mem s₁ a → mem s₂ a
-  union : {α : Type u} → S α → S α → S α
-  inter : {α : Type u} → S α → S α → S α
-  sdiff : {α : Type u} → S α → S α → S α
-  symmDiff : {α : Type u} → S α → S α → S α :=
-    fun s₁ s₂ => union (sdiff s₁ s₂) (sdiff s₂ s₁)
-  disjoint : {α : Type u} → S α → S α → Prop :=
-    fun s₁ s₂ => ∀ a, ¬(mem (inter s₁ s₂) a)
-  -- filter {α : Type u} (s : S α) (pred : α → Bool) : S α
-  filter : {α : Type u} → (s : S α) → (pred : α → Bool) → S α
-  ofList : {α : Type u} → List α → (S α) :=
-    fun l => l.foldl (fun a s => insert a s) empty
-  isEmpty : S α → Prop :=
-    fun s => s = empty
-  isSingleton : {α : Type u} → S α → Prop :=
-    fun s => ∃ a, s = singleton a
   findUniqueMinimal {α : Type u} [Inhabited α] : (S α) → (r : α → α → Bool) → α
   findUniqueMaximal {α : Type u} [Inhabited α] : (S α) → (r : α → α → Bool) → α
   all : {α : Type u} → (S α) → (α → Bool) → Prop :=
     fun s p => ∀ a, mem s a → p a
   any : {α : Type u} → (S α) → (α → Bool) → Prop :=
     fun s p => ∃ a, mem s a ∧ p a
-  filterMap : {α β : Type u} → (α → Option β) → (S α) → S β
   setIntRange : {α : Type u} → (a b : Int) → S α
-
-  fromSeq : {α : Type u} → Seq α → S α
-
-#exit
-
--- export VSetLikeF (symmDiff disjoint filter ofList)
-
-namespace VSetLikeF
-
-variable {S : Type u → Type v} [VSetLikeF S]
-
-instance instEmptyCollection : EmptyCollection (S α) := ⟨empty⟩
-instance instInhabited : Inhabited (S α) := ⟨∅⟩
-instance instSingleton : Singleton α (S α) := ⟨singleton⟩
-instance instMembership : Membership α (S α) := ⟨mem⟩
-instance instInsert : Insert α (S α) := ⟨fun a s => insert s a⟩
-instance instHasSubset : HasSubset (S α) := ⟨subset⟩
-instance instLE : LE (S α) := ⟨subset⟩
-instance instLT : LT (S α) := ⟨fun s₁ s₂ => s₁ ⊆ s₂ ∧ ¬(s₂ ⊆ s₁)⟩
-instance instUnion : Union (S α) := ⟨union⟩
-instance instInter : Inter (S α) := ⟨inter⟩
-instance instSDiff : SDiff (S α) := ⟨sdiff⟩
-instance instHAdd : HAdd (S α) (S α) (S α) := ⟨(· ∪ ·)⟩
-instance instHSub : HSub (S α) (S α) (S α) := ⟨(· \ ·)⟩
-instance instHMul : HMul (S α) (S α) (S α) := ⟨(· ∩ ·)⟩
-instance instHAddSingleton : HAdd (S α) α (S α) := ⟨fun s a => insert s a⟩
-instance instHSubSingleton : HSub (S α) α (S α) := ⟨fun s a => remove a s⟩
-instance instCoeList : Coe (List α) (S α) := ⟨ofList⟩
-
-end VSetLikeF
-
-class VSetF (S : Type u → Type v)
-  extends
-    VSetLikeF S
-  where
-  /-- The cardinality of the set. -/
-  card : S α → Nat
-  /-- Dedup-ed list. Ordering not specified. -/
-  toList : {α : Type u} → S α → List α
-  fold {α : Type u} {β : Type u} (s : S α) (init : β) (f : β → α → β) : β
 
 class VSetInfF (S : Type u → Type v)
   extends VSetLikeF S
@@ -466,35 +556,6 @@ class VSetInfF (S : Type u → Type v)
   fold {α : Type u} {β : Type u} (s : S α) (init : β) (f : β → α → β) : (h_finite : isFinite s) → β
   isFull : S α → Prop := fun s => s = full
 
-open VSetLikeF in
-class LawfulVSetLikeF (S : Type u → Type v) [VSetLikeF S]
-  extends
-    LawfulFunctor S
-  where
-  protected ext (s₁ s₂ : S α) : (∀ (x : α), x ∈ s₁ ↔ x ∈ s₂) → s₁ = s₂
-  not_mem_empty : ∀ (a : α), a ∉ (∅ : S α)
-  mem_insert_iff {a b : α} {s : S α} : b ∈ (s + a) ↔ b = a ∨ b ∈ s
-  mem_remove_iff {a b : α} {s : S α} : b ∈ (s - a) ↔ b ≠ a ∧ b ∈ s
-  mem_singleton_iff {a b : α} : b ∈ ({a} : S α) ↔ b = a
-  -- choose_mem {α : Type u} [Inhabited α] : ∀ (s : S α) (h : ∃ x, x ∈ s), choose s h ∈ s
-  choose_mem {α : Type u} [Inhabited α] : ∀ (s : S α), (h : ∃ x, x ∈ s) → choose s ∈ s
-  subset_iff {s₁ s₂ : S α} : s₁ ⊆ s₂ ↔ ∀ a, a ∈ s₁ → a ∈ s₂
-  mem_union_iff  {a : α} {s₁ s₂ : S α} : a ∈ s₁ ∪ s₂ ↔ a ∈ s₁ ∨ a ∈ s₂
-  mem_inter_iff  {a : α} {s₁ s₂ : S α} : a ∈ s₁ ∩ s₂ ↔ a ∈ s₁ ∧ a ∈ s₂
-  mem_sdiff_iff  {a : α} {s₁ s₂ : S α} : a ∈ s₁ \ s₂ ↔ a ∈ s₁ ∧ a ∉ s₂
-  mem_symmDiff_iff {a : α} {s₁ s₂ : S α} : a ∈ symmDiff s₁ s₂ ↔ (a ∈ s₁ \ s₂ ∨ a ∈ s₂ \ s₁)
-  disjoint_iff {s₁ s₂ : S α} : disjoint s₁ s₂ ↔ ∀ a, a ∉ s₁ ∩ s₂
-  mem_filter_iff {p : α → Bool} {s : S α} {a : α} : a ∈ filter s p ↔ a ∈ s ∧ p a
-  mem_ofList_iff {a : α} {l : List α} : a ∈ (ofList l : S α) ↔ a ∈ l
-  mem_map_iff {f : α → β} {s : S α} {b : β}
-    : b ∈ f <$> s ↔ ∃ a, a ∈ s ∧ f a = b
-  mem_filterMap_iff {α β : Type u} {f : α → Option β} {s : S α} {b : β}
-    : b ∈ filterMap f s ↔ ∃ a, a ∈ s ∧ f a = some b
-
-open LawfulVSetLikeF in
-attribute [simp] not_mem_empty mem_singleton_iff mem_ofList_iff
-attribute [ext] LawfulVSetLikeF.ext
-
 open VSetLikeF VSetF in
 class LawfulVSetF (S : Type u → Type v) [VSetF S]
   extends
@@ -507,9 +568,5 @@ class LawfulVSetF (S : Type u → Type v) [VSetF S]
   fold_empty : ∀ {β : Type u} (f : β → α → β) (init : β), fold (∅ : S α) init f = init
   fold_mem : ∀ {β : Type u} (f : β → α → β) [FoldCommutative f] (init : β) {s : S α} (a : α),
       a ∈ s → fold s init f = fold (s - a) (f init a) f
-
-open LawfulVSetF in
-attribute [simp] card_empty fold_empty
-
 
 end Vstd
